coq/examples/reduction_gen.v
@@ -8,11 +8,11 @@ Module MS := MIRSemantics.
 Module Reduction_gen.
 
 Definition prog : list M.stmt :=
-  [ M.SStoreShared (M.EPtrAdd (M.EVar "_1") (M.EVar "_6)")) (M.EVar "_3") M.TyF32;
+  [ M.SStoreShared (M.EPtrAdd (M.EVar "_1") (M.EVar "_6")) (M.EVar "_3") M.TyF32;
     M.SBarrierShared;
-    M.SFor "_loop_counter" 3 [ M.SLoadShared "_18" (M.EPtrAdd (M.EVar "_1") (M.EVar "_20)")) M.TyF32;
-        M.SLoadShared "_21" (M.EPtrAdd (M.EVar "_1") (M.EVar "_23)")) M.TyF32;
-        M.SStoreShared (M.EPtrAdd (M.EVar "_1") (M.EVar "_27)")) (M.EAdd (M.EVar "_18") (M.EVar "_21")) M.TyF32;
+    M.SFor "_loop_counter" 3 [ M.SLoadShared "_18" (M.EPtrAdd (M.EVar "_1") (M.EVar "_20")) M.TyF32;
+        M.SLoadShared "_21" (M.EPtrAdd (M.EVar "_1") (M.EVar "_23")) M.TyF32;
+        M.SStoreShared (M.EPtrAdd (M.EVar "_1") (M.EVar "_27")) (M.EAdd (M.EVar "_18") (M.EVar "_21")) M.TyF32;
         M.SBarrierShared ] ].
 
 End Reduction_gen.
